src/AbstractDomain.v
@@ -1,0 +1,20 @@
+Require Export Coq.Sets.Ensembles.
+From Coq Require Import ssrbool.
+
+(* The abstract domain *)
+Class adom (concrete_state abstract_state: Type) :=
+  {
+    le : abstract_state -> abstract_state -> bool;
+    bot : abstract_state;
+    top : abstract_state;
+    join : abstract_state -> abstract_state -> abstract_state;
+
+    gamma : abstract_state -> Ensemble concrete_state;
+
+    le_refl: forall a, le a a;
+    le_trans: forall a1 a2 a3, le a1 a2 -> le a2 a3 -> le a1 a3;
+    gamma_monotone : forall a1 a2, le a1 a2 -> Included concrete_state (gamma a1) (gamma a2);
+    gamma_top : forall x, Ensembles.In concrete_state (gamma top) x;
+    join_sound_l : forall a1 a2, le a1 (join a1 a2);
+    join_sound_r : forall a1 a2, le a2 (join a1 a2);
+  }.
